src/PermProgLoop.v
@@ -1,0 +1,620 @@
+Require Import Pred Mem Word Arith.
+Require Import Nomega NArith Omega List.
+Require Import Morphisms FunctionalExtensionality ProofIrrelevance.
+Require Export PermInstr.
+
+Set Implicit Arguments.
+
+Record For_args (L : Type) := {
+  For_args_i : waddr;
+  For_args_n : waddr;
+  For_args_l : L
+}.
+
+Theorem for_args_wf: forall L,
+  well_founded (fun a b => wlt a.(@For_args_n L) b.(@For_args_n L)).
+Proof.
+  intros.
+  apply well_founded_lt_compat with (f:=fun a => wordToNat (@For_args_n L a)).
+  intros.
+  apply wlt_lt; auto.
+Qed.
+
+Lemma word_minus_1 : forall sz (w: word sz),
+    w <> $ 0 ->
+    (w ^- $1 < w)%word.
+Proof.
+  intros.
+  apply weq_minus1_wlt; auto.
+Qed.
+
+Definition For_ (L : Type) (G : Type) (f : waddr -> L -> prog L)
+                (i n : waddr)
+                (nocrash : G -> waddr -> L -> block_mem -> hashmap -> rawpred)
+                (crashed : G -> block_mem -> hashmap -> rawpred)
+                (l : L) : prog L.
+Proof.
+  refine (Fix (@for_args_wf L) (fun _ => prog L)
+          (fun args For_ => _)
+          {| For_args_i := i; For_args_n := n; For_args_l := l |}).
+  clear i n l.
+  destruct args.
+  refine (if weq For_args_n0 $0 then Ret For_args_l0 else _).
+  refine (l' <- (f For_args_i0 For_args_l0);; _).
+  refine (For_ {| For_args_i := For_args_i0 ^+ $1;
+                  For_args_n := For_args_n0 ^- $1;
+                  For_args_l := l' |} _).
+
+  simpl.
+  apply word_minus_1; auto.
+Defined.
+
+Lemma For_step: forall L G (f: waddr -> L -> prog L) i n l nocrash crashed,
+  @For_ L G f i n nocrash crashed l =
+    if weq n $0
+    then Ret l
+    else l' <- (f i l);;
+         @For_ L G f
+             (i ^+ $1)
+             (n ^- $1)
+             nocrash crashed l'.
+Proof.
+  intros.
+  unfold For_.
+  rewrite Fix_eq.
+  simpl.
+
+  destruct (weq n $0); f_equal.
+
+  intros.
+
+  match goal with
+  | [ |- context[match ?x with _ => _ end] ] =>
+     destruct x; f_equal
+  end.
+
+  match goal with
+  | [ |- context[match ?x with _ => _ end] ] =>
+     destruct x; try reflexivity
+  end.
+
+  apply f_equal.
+  apply functional_extensionality; auto.
+Qed.
+
+Theorem for_ok':
+  forall T (n i : waddr)
+         (L : Type) (G : Type)
+         (f: waddr -> L -> prog L) (rx: L -> prog T)
+         (nocrash : G -> waddr -> L -> block_mem -> hashmap -> rawpred)
+         (crashed : G -> block_mem -> hashmap -> rawpred)
+         (li : L) pr,
+    {{ pr | fun done crash bm hm =>
+      (exists F (g:G) bm' hm',
+      F * nocrash g i li bm hm * [[ bm' c= bm ]] *
+      [[ exists l, hashmap_subset l hm' hm ]] *
+      [[forall m lm rxm,
+      (i <= m)%word ->
+      (m < n ^+ i)%word ->
+      (forall lSm,
+       {{ pr |  fun  done' crash' bm'' hm'' => F * nocrash g (m ^+ $1) lSm bm'' hm'' *
+          [[ exists l, hashmap_subset l hm' hm'' ]] * [[ bm' c= bm'' ]] *
+          [[ done' = done ]] * [[ crash' = crash ]]
+       }} rxm lSm) ->
+      {{ pr | fun done' crash' bm'' hm'' => F * nocrash g m lm bm'' hm'' *
+          [[ exists l, hashmap_subset l hm' hm'' ]] * [[ bm' c= bm'' ]] *
+          [[ done' = done ]] * [[ crash' = crash ]]
+      }} Bind (f m lm) rxm]] *
+     [[forall lfinal,
+       {{ pr | fun done' crash' bm'' hm''  => F * nocrash g (n ^+ i) lfinal bm'' hm'' *
+          [[ exists l, hashmap_subset l hm' hm'' ]] * [[ bm' c= bm'' ]] *
+          [[ done' = done ]] * [[ crash' = crash ]]
+       }} rx lfinal]] *
+     [[wordToNat i + wordToNat n = wordToNat (i ^+ n)]] *
+     [[forall bm'' hm'',
+         F * crashed g bm'' hm'' * [[ exists l, hashmap_subset l hm' hm'' ]] *
+         [[ bm' c= bm'' ]] =p=> crash bm'' hm'' ]])%pred
+  }} Bind (For_ f i n nocrash crashed li) rx.
+Proof.
+  intro T.
+  wlt_ind.
+
+  intros.
+  apply corr2_exists; intros.
+  apply corr2_exists; intros.
+  apply corr2_exists; intros.
+  apply corr2_exists; intros.
+  case_eq (weq x $0); intros; subst.
+
+  - eapply pimpl_pre2; intros; repeat ( apply sep_star_lift_l; intros ).
+    + unfold pimpl, lift; intros.
+      rewrite For_step.
+      eapply pimpl_ok2.
+      simpl; monad_simpl; eauto.
+      apply ret_secure'.
+      intros.
+      apply pimpl_refl.
+    + fold (wzero addrlen). ring_simplify (wzero addrlen ^+ i). cancel.
+      eassign (fun bm hm => (nocrash a0 i li bm hm * a)%pred); simpl; cancel.
+      eapply pimpl_ok2; eauto. intros; simpl. safecancel.
+      fold (wzero addrlen). ring_simplify (wzero addrlen ^+ i). cancel.
+      eexists; eapply hashmap_subset_trans; eauto.
+      cancel; eauto.
+
+  - eapply pimpl_pre2; intros; repeat ( apply sep_star_lift_l; intros ).
+    + assert (wordToNat x <> 0).
+      unfold not in *; intros; apply n.
+      rewrite <- H7; rewrite natToWord_wordToNat; auto.
+
+      unfold pimpl, lift; intros.
+      rewrite For_step.
+      rewrite H0.
+      monad_simpl.
+      apply H4.
+
+      apply eq_le; auto.
+      rewrite wplus_comm.
+      apply lt_wlt.
+      omega.
+
+      intros.
+      eapply pimpl_ok2.
+      apply H.
+
+      apply word_minus_1; auto.
+
+      intros.
+      apply pimpl_exists_r; exists a.
+      apply pimpl_exists_r; exists a0.
+      apply pimpl_exists_r; exists a1.
+      ring_simplify (i ^+ $1 ^+ (x ^- $1)).
+      ring_simplify (x ^- $1 ^+ (i ^+ $1)).
+      cancel.
+      eauto.
+
+      subst; apply H4; eauto.
+      intros; apply H10; clear H10.
+      apply wlt_lt in H14.
+      unfold wlt.
+      repeat rewrite wordToN_nat.
+      apply Nlt_in.
+      repeat rewrite Nat2N.id.
+      rewrite wplus_alt.
+      unfold wplusN, wordBinN.
+      simpl (wordToNat $1).
+      rewrite wordToNat_natToWord_idempotent'.
+      omega.
+      eapply Nat.le_lt_trans; [| apply (wordToNat_bound (i ^+ x)) ]; omega.
+
+      rewrite wminus_Alt.
+      rewrite wminus_Alt2.
+      repeat rewrite wplus_alt.
+      repeat unfold wplusN, wordBinN.
+
+      simpl (wordToNat $1).
+      repeat rewrite wordToNat_natToWord_idempotent'.
+      omega.
+      rewrite H2; apply wordToNat_bound.
+
+      eapply Nat.le_lt_trans; [| apply (wordToNat_bound x) ]; omega.
+      eapply Nat.le_lt_trans; [| apply (wordToNat_bound (i ^+ x)) ]; omega.
+
+      unfold not; intros; apply H7.
+      assert (wordToNat x < 1); [| omega ].
+      apply wlt_lt in H10; simpl in H10; auto.
+    + cancel; eauto.
+Qed.
+
+Theorem for_ok:
+  forall T (n : waddr)
+         (L : Type) (G : Type)
+         f (rx: _ -> prog T)
+         (nocrash : G -> waddr -> L -> block_mem -> hashmap -> rawpred)
+         (crashed : G -> block_mem -> hashmap -> rawpred)
+         (li : L) pr,
+    {{ pr | fun done crash bm hm =>
+         (exists F (g:G) bm' hm', F * nocrash g $0 li bm hm
+   * [[ exists l, hashmap_subset l hm' hm ]] * [[ bm' c= bm ]]
+   * [[forall m lm rxm,
+      (m < n)%word ->
+      (forall lSm,
+       {{ pr | fun done' crash' bm'' hm'' => F * nocrash g (m ^+ $1) lSm bm'' hm'' *
+          [[ exists l, hashmap_subset l hm' hm'' ]] * [[ bm' c= bm'' ]] *
+          [[ done' = done ]] * [[ crash' = crash ]]
+       }} rxm lSm) ->
+      {{ pr | fun done' crash' bm'' hm'' => F * nocrash g m lm bm'' hm'' *
+          [[ exists l, hashmap_subset l hm' hm'' ]] * [[ bm' c= bm'' ]] *
+          [[ done' = done ]] * [[ crash' = crash ]]
+      }} Bind (f m lm) rxm]]
+   * [[forall lfinal,
+       {{ pr | fun done' crash' bm'' hm'' => F * nocrash g n lfinal bm'' hm'' *
+          [[ exists l, hashmap_subset l hm' hm'' ]] * [[ bm' c= bm'' ]] *
+          [[ done' = done ]] * [[ crash' = crash ]]
+       }} rx lfinal]]
+   * [[forall bm'' hm'',
+         F * crashed g bm'' hm'' * [[ exists l, hashmap_subset l hm' hm'' ]] *
+         [[ bm' c= bm'' ]] =p=> crash bm'' hm'' ]])%pred
+  }} Bind (For_ f $0 n nocrash crashed li) rx.
+Proof.
+  intros.
+  eapply pimpl_ok2.
+  apply for_ok'.
+  fold (wzero addrlen); ring_simplify (wzero addrlen ^+ n).
+  simpl (wordToNat (wzero addrlen)); replace (0 + wordToNat n) with (wordToNat n) by omega.
+  ring_simplify (n ^+ wzero addrlen).
+  safecancel.
+  cancel; apply pimpl_refl.
+  eassign bm'; cancel.
+  eauto.
+  eauto.
+  eauto.
+  rewrite <- H1; cancel; eauto.
+  Unshelve.
+  unfold EqDec; intros; apply handle_eq_dec.
+Qed.
+
+Hint Extern 1 ({{_ | _}} Bind (For_ _ _ _ _ _ _) _) => apply for_ok : prog.
+
+Notation "'For' i < n 'Ghost' [ g1 .. g2 ] 'Loopvar' [ l1 .. l2 ] 'Invariant' nocrash 'OnCrash' crashed 'Begin' body 'Rof'" :=
+  (For_ (fun i =>
+          (pair_args_helper (fun l1 => ..
+            (pair_args_helper (fun l2 (_:unit) => body))
+          ..)))
+        $0 n
+        (pair_args_helper (fun bm0 =>
+        (pair_args_helper (fun g1 => .. (pair_args_helper (fun g2 (_:unit) =>
+         fun i =>
+          (pair_args_helper (fun l1 => .. (pair_args_helper (fun l2 (_:unit) =>
+           fun bm hm => ([[ bm = bm0 ]] * nocrash)%pred)) ..))
+        )) .. ))))
+        (pair_args_helper (fun g1 => .. (pair_args_helper (fun g2 (_:unit) =>
+         fun bm hm => crashed%pred)) .. )))
+  (at level 9, i at level 0, n at level 0,
+   g1 closed binder, g2 closed binder,
+   l1 closed binder, l2 closed binder,
+   body at level 9).
+
+
+Notation "'For' i < n 'Blockmem' bm 'Hashmap' hm 'Ghost' [ g1 .. g2 ] 'Loopvar' [ l1 .. l2 ] 'Invariant' nocrash 'OnCrash' crashed 'Begin' body 'Rof'" :=
+  (For_ (fun i =>
+          (pair_args_helper (fun l1 => ..
+            (pair_args_helper (fun l2 (_:unit) => body))
+          ..)))
+        $0 n
+        (pair_args_helper (fun bm0 =>
+        (pair_args_helper (fun g1 => .. (pair_args_helper (fun g2 (_:unit) =>
+         fun i =>
+          (pair_args_helper (fun l1 => .. (pair_args_helper (fun l2 (_:unit) =>
+           fun bm hm => ([[ bm = bm0 ]] * nocrash)%pred)) ..))
+        )) .. ))))
+        (pair_args_helper (fun g1 => .. (pair_args_helper (fun g2 (_:unit) =>
+         fun bm hm => crashed%pred)) .. )))
+  (at level 9, i at level 0, n at level 0,
+   g1 closed binder, g2 closed binder,
+   l1 closed binder, l2 closed binder,
+   body at level 9).
+
+
+Fixpoint ForN_  (L : Type) (G : Type) (f : nat -> L -> prog L)
+                (i n : nat)
+                (nocrash : G -> nat -> L -> block_mem -> hashmap -> rawpred)
+                (crashed : G -> block_mem -> hashmap -> rawpred)
+                (l : L) : prog L :=
+  match n with
+  | 0 =>   Ret l
+  | S m => l' <- f i l;;  ForN_ f (S i) m nocrash crashed l'
+  end.
+
+
+Theorem forN_ok':
+  forall T (n i : nat)
+         (L : Type) (G : Type)
+         f (rx: _ -> prog T)
+         (nocrash : G -> nat -> L -> block_mem -> hashmap -> pred)
+         (crashed : G -> block_mem -> hashmap -> pred)
+         (li : L) pr,
+  {{ pr | fun done crash bm hm => (exists F (g:G) bm' hm', F * nocrash g i li bm hm
+   * [[ exists l, hashmap_subset l hm' hm ]] * [[ bm' c= bm ]]
+   * [[forall m lm rxm,
+      i <= m ->
+      m < n + i ->
+      (forall lSm,
+       {{ pr | fun done' crash' bm'' hm'' => F * nocrash g (S m) lSm bm'' hm'' *
+          [[ exists l, hashmap_subset l hm' hm'' ]] * [[ bm' c= bm'' ]] *
+          [[ done' = done ]] * [[ crash' = crash ]]
+       }} rxm lSm) ->
+      {{ pr | fun done' crash' bm'' hm'' => F * nocrash g m lm bm'' hm'' *
+          [[ exists l, hashmap_subset l hm' hm'' ]] * [[ bm' c= bm'' ]] *
+          [[ done' = done ]] * [[ crash' = crash ]]
+      }} Bind (f m lm) rxm]]
+   * [[forall lfinal,
+       {{ pr | fun done' crash' bm'' hm''=> F * nocrash g (n + i) lfinal bm'' hm'' *
+          [[ exists l, hashmap_subset l hm' hm'' ]] * [[ bm' c= bm'' ]] *
+          [[ done' = done ]] * [[ crash' = crash ]]
+       }} rx lfinal]]
+   * [[forall bm'' hm'',
+        F * crashed g bm'' hm'' *
+        [[ exists l, hashmap_subset l hm' hm'' ]] * [[ bm' c= bm'' ]] =p=> crash bm'' hm'' ]])%pred
+  }} Bind (ForN_ f i n nocrash crashed li) rx.
+Proof.
+  induction n; intros;
+    apply corr2_exists; intros;
+    apply corr2_exists; intros;
+    apply corr2_exists; intros;
+    apply corr2_exists; intros.
+  - eapply pimpl_pre2; intros; repeat ( apply sep_star_lift_l; intros ).
+    + simpl.
+      unfold pimpl, lift; intros.
+      eapply pimpl_ok2; monad_simpl.
+      apply ret_secure'.
+      intros.
+      apply pimpl_refl.
+    + simpl. cancel.
+      eassign (fun bm hm => nocrash a0 i li bm hm * a)%pred.
+      apply pimpl_refl.
+      eapply pimpl_ok2; eauto.
+      intros; cancel.
+      eexists; eapply hashmap_subset_trans; eauto.
+      cancel; auto.
+  - eapply pimpl_pre2; intros; repeat ( apply sep_star_lift_l; intros ).
+    + simpl.
+      unfold pimpl, lift; intros.
+
+      eapply pimpl_ok2; monad_simpl.
+      apply H1. omega. omega.
+      intros.
+      eapply pimpl_ok2.
+      eapply IHn.
+      safecancel.
+      cancel.
+      apply pimpl_refl.
+      eauto.
+      eassign a1; cancel.
+
+      apply H1.
+      omega.
+      omega.
+      auto.
+
+      replace (n + S i) with (S (n + i)) by omega.
+      eauto.
+
+      rewrite <- H; cancel; eauto.
+      intros; apply pimpl_refl.
+    + cancel; eauto.
+ Unshelve.
+ unfold EqDec; apply handle_eq_dec.     
+Qed.
+
+Theorem forN_ok:
+  forall (n : nat)
+         T (L : Type) (G : Type)
+         f (rx: _ -> prog T)
+         (nocrash : G -> nat -> L -> block_mem -> hashmap -> pred)
+         (crashed : G -> block_mem -> hashmap -> pred)
+         (li : L) pr,
+  {{ pr | fun done crash bm hm => (exists F (g:G) bm' hm', F * nocrash g 0 li bm hm
+   * [[ exists l, hashmap_subset l hm' hm ]] * [[ bm' c= bm ]]
+   * [[forall m lm rxm,
+      m < n ->
+      (forall lSm,
+       {{ pr | fun done' crash' bm'' hm'' => F * nocrash g (S m) lSm bm'' hm'' *
+          [[ exists l, hashmap_subset l hm' hm'' ]] * [[ bm' c= bm'' ]] *
+          [[ done' = done ]] * [[ crash' = crash ]]
+       }} rxm lSm) ->
+      {{ pr | fun done' crash' bm'' hm'' => F * nocrash g m lm bm'' hm'' *
+          [[ exists l, hashmap_subset l hm' hm'' ]] * [[ bm' c= bm'' ]] *
+          [[ done' = done ]] * [[ crash' = crash ]]
+      }} Bind (f m lm) rxm]]
+   * [[forall lfinal,
+       {{ pr | fun done' crash' bm'' hm'' => F * nocrash g n lfinal bm'' hm'' *
+          [[ exists l, hashmap_subset l hm' hm'' ]] * [[ bm' c= bm'' ]] *
+          [[ done' = done ]] * [[ crash' = crash ]]
+       }} rx lfinal]]
+   * [[forall bm'' hm'',
+         F * crashed g bm'' hm'' * [[ exists l, hashmap_subset l hm' hm'' ]] *
+         [[ bm' c= bm'' ]] =p=> crash bm'' hm'' ]])%pred
+  }} Bind (ForN_ f 0 n nocrash crashed li) rx.
+Proof.
+  intros.
+  eapply pimpl_ok2.
+  apply forN_ok'.
+  safecancel.
+  cancel; apply pimpl_refl.
+  eauto.
+  eassign bm'; cancel.
+  apply H3.
+  omega.
+  auto.
+  eapply pimpl_ok2.
+  eauto.
+  replace (n + 0) with n by omega; auto.
+  rewrite <- H1; cancel; eauto.
+  Unshelve.
+  unfold EqDec; apply handle_eq_dec.
+Qed.
+
+Hint Extern 1 ({{_ | _}} Bind (ForN_ _ _ _ _ _ _) _) => apply forN_ok : prog.
+
+Notation "'ForN' i < n 'Ghost' [ g1 .. g2 ] 'Loopvar' [ l1 .. l2 ] 'Invariant' nocrash 'OnCrash' crashed 'Begin' body 'Rof'" :=
+  (ForN_ (fun i =>
+          (pair_args_helper (fun l1 => ..
+            (pair_args_helper (fun l2 (_:unit) => body))
+          ..)))
+        0 n
+        (pair_args_helper (fun bm0 =>
+        (pair_args_helper (fun g1 => .. (pair_args_helper (fun g2 (_:unit) =>
+         fun i =>
+          (pair_args_helper (fun l1 => .. (pair_args_helper (fun l2 (_:unit) =>
+           fun bm hm => ([[ bm = bm0 ]] * nocrash)%pred)) ..))
+        )) .. ))))
+        (pair_args_helper (fun bm0 =>
+        (pair_args_helper (fun g1 => .. (pair_args_helper (fun g2 (_:unit) =>
+         fun bm hm => crashed%pred)) .. )))))
+  (at level 9, i at level 0, n at level 0,
+   g1 closed binder, g2 closed binder,
+   l1 closed binder, l2 closed binder,
+   body at level 9).
+
+Notation "'ForN' i < n 'Blockmem' bm 'Hashmap' hm 'Ghost' [ g1 .. g2 ] 'Loopvar' [ l1 .. l2 ] 'Invariant' nocrash 'OnCrash' crashed 'Begin' body 'Rof'" :=
+  (ForN_ (fun i =>
+          (pair_args_helper (fun l1 => ..
+            (pair_args_helper (fun l2 (_:unit) => body))
+          ..)))
+        0 n
+        (pair_args_helper (fun bm0 =>
+        (pair_args_helper (fun g1 => .. (pair_args_helper (fun g2 (_:unit) =>
+         fun i =>
+          (pair_args_helper (fun l1 => .. (pair_args_helper (fun l2 (_:unit) =>
+           fun bm hm => ([[ bm = bm0 ]] * nocrash)%pred)) ..))
+        )) .. ))))
+        (pair_args_helper (fun bm0 =>
+        (pair_args_helper (fun g1 => .. (pair_args_helper (fun g2 (_:unit) =>
+         fun bm hm => crashed%pred)) .. )))))
+  (at level 9, i at level 0, n at level 0,
+   g1 closed binder, g2 closed binder,
+   l1 closed binder, l2 closed binder,
+   body at level 9).
+
+Notation "'ForN' x <= i < n 'Blockmem' bm 'Hashmap' hm 'Ghost' [ g1 .. g2 ] 'Loopvar' [ l1 .. l2 ] 'Invariant' nocrash 'OnCrash' crashed 'Begin' body 'Rof'" :=
+  (ForN_ (fun i =>
+          (pair_args_helper (fun l1 => ..
+            (pair_args_helper (fun l2 (_:unit) => body))
+          ..)))
+        x (n - x)
+        (pair_args_helper (fun bm0 =>
+        (pair_args_helper (fun g1 => .. (pair_args_helper (fun g2 (_:unit) =>
+         fun i =>
+          (pair_args_helper (fun l1 => .. (pair_args_helper (fun l2 (_:unit) =>
+           fun bm hm => ([[ bm = bm0 ]] * nocrash)%pred)) ..))
+        )) .. ))))
+        (pair_args_helper (fun bm0 =>
+        (pair_args_helper (fun g1 => .. (pair_args_helper (fun g2 (_:unit) =>
+         fun bm hm => crashed%pred)) .. )))))
+  (at level 9, i at level 0, n at level 0, x at level 0,
+   g1 closed binder, g2 closed binder,
+   l1 closed binder, l2 closed binder,
+   body at level 9).
+
+Fixpoint ForEach_ (ITEM : Type)
+                (L : Type) (G : Type) (f : ITEM -> L -> prog L)
+                (lst : list ITEM)
+                (nocrash : G -> list ITEM -> L -> block_mem -> hashmap -> rawpred)
+                (crashed : G -> block_mem -> hashmap -> rawpred)
+                (l : L) : prog L :=
+  match lst with
+  | nil => Ret l
+  | elem :: lst' =>
+    l' <- f elem l;;
+    ForEach_ f lst' nocrash crashed l'
+  end.
+
+Theorem foreach_ok:
+  forall T ITEM (lst : list ITEM)
+         (L : Type) (G : Type)
+         f (rx: _ -> prog T)
+         (nocrash : G -> list ITEM -> L -> block_mem -> hashmap -> pred)
+         (crashed : G -> block_mem -> hashmap -> pred)
+         (li : L) pr,
+  {{ pr | fun done crash bm hm => (exists F (g:G) bm' hm', F * nocrash g lst li bm hm
+   * [[ exists l, hashmap_subset l hm' hm ]] * [[ bm' c= bm ]]
+   * [[forall elem lst' lm rxm,
+      (forall lSm,
+       {{ pr | fun done' crash' bm'' hm'' => F * nocrash g lst' lSm bm'' hm'' *
+          [[ exists l, hashmap_subset l hm' hm'' ]] * [[ bm' c= bm'' ]] *
+          [[ done' = done ]]  * [[ crash' = crash ]]
+       }} rxm lSm) ->
+      {{ pr | fun done' crash' bm'' hm'' => F * nocrash g (elem :: lst') lm bm'' hm'' *
+         [[ exists l, hashmap_subset l hm' hm'' ]] * [[ bm' c= bm'' ]] *
+         [[ exists prefix, prefix ++ elem :: lst' = lst ]] *
+         [[ done' = done ]] * [[ crash' = crash ]]
+      }} Bind (f elem lm) rxm]]
+   * [[forall lfinal,
+       {{ pr | fun done' crash' bm'' hm'' => F * nocrash g nil lfinal bm'' hm'' *
+          [[ exists l, hashmap_subset l hm' hm'' ]] * [[ bm' c= bm'' ]] *
+          [[ done' = done ]] * [[ crash' = crash ]]
+       }} rx lfinal]]
+   * [[forall bm'' hm'',
+         F * crashed g bm'' hm'' * [[ exists l, hashmap_subset l hm' hm'' ]] *
+         [[ bm' c= bm ]] =p=> crash bm'' hm'' ]])%pred
+  }} Bind (ForEach_ f lst nocrash crashed li) rx.
+Proof.
+  intros ITEM.
+  induction lst; intros;
+    apply corr2_exists; intros;
+    apply corr2_exists; intros;
+    apply corr2_exists; intros;
+    apply corr2_exists; intros.
+
+  - eapply pimpl_pre2; intros; repeat ( apply sep_star_lift_l; intros ).
+    + simpl.
+      unfold pimpl, lift; intros.
+      eapply pimpl_ok2; monad_simpl.
+      apply ret_secure'.
+      intros.
+      apply pimpl_refl.
+    + safecancel.
+      eassign (fun bm hm => nocrash a0 nil li bm hm * a)%pred.
+      apply pimpl_refl.
+      eapply pimpl_ok2; eauto.
+      cancel; eauto.
+      eexists; eapply hashmap_subset_trans; eauto.
+      cancel; eauto.
+  - eapply pimpl_pre2; intros; repeat ( apply sep_star_lift_l; intros ).
+    + simpl.
+      unfold pimpl, lift; intros.
+      monad_simpl; apply H1.
+      intros.
+      eapply pimpl_ok2.
+      apply IHlst.
+      safecancel.
+      eassign lst.
+      cancel; apply pimpl_refl.
+      eauto.
+      eassign a2; cancel.
+      eapply pimpl_ok2.
+      apply H1.
+      intros.
+      auto.
+      cancel; eauto.
+      exists (a :: prefix); auto.
+      auto.
+      rewrite <- H; cancel; eauto.
+    + cancel.
+      eauto.
+      exists nil; auto.
+ Unshelve.
+ unfold EqDec; apply handle_eq_dec.     
+Qed.
+
+Hint Extern 1 ({{_ | _}} Bind (ForEach_ _ _ _ _ _) _) => apply foreach_ok : prog.
+
+Notation "'ForEach' elem rest lst 'Ghost' [ g1 .. g2 ] 'Loopvar' [ l1 .. l2 ] 'Invariant' nocrash 'OnCrash' crashed 'Begin' body 'Rof'" :=
+  (ForEach_ (fun elem => (pair_args_helper (fun l1 => .. (pair_args_helper (fun l2 (_:unit) => body)) ..)))
+        lst
+        (pair_args_helper (fun bm0 =>
+        (pair_args_helper (fun g1 => .. (pair_args_helper (fun g2 (_:unit) =>
+         fun rest => (pair_args_helper (fun l1 => .. (pair_args_helper (fun l2 (_:unit) =>
+         fun bm hm => ([[ bm = bm0 ]] * nocrash)%pred)) ..))  )) .. ))))
+        (pair_args_helper (fun bm0 =>
+        (pair_args_helper (fun g1 => .. (pair_args_helper (fun g2 (_:unit) =>
+         fun bm hm => crashed%pred)) .. )))))
+  (at level 9, elem at level 0, rest at level 0,
+   g1 closed binder, g2 closed binder,
+   l1 closed binder, l2 closed binder,
+   body at level 9).
+
+Notation "'ForEach' elem rest lst 'Hashmap' hm 'Ghost' [ g1 .. g2 ] 'Loopvar' [ l1 .. l2 ] 'Invariant' nocrash 'OnCrash' crashed 'Begin' body 'Rof'" :=
+  (ForEach_ (fun elem => (pair_args_helper (fun l1 => .. (pair_args_helper (fun l2 (_:unit) => body)) ..)))
+        lst
+        (pair_args_helper (fun bm0 =>
+        (pair_args_helper (fun g1 => .. (pair_args_helper (fun g2 (_:unit) =>
+         fun rest => (pair_args_helper (fun l1 => .. (pair_args_helper (fun l2 (_:unit) =>
+         fun bm hm => ([[ bm = bm0 ]] * nocrash)%pred)) ..))  )) .. ))))
+        (pair_args_helper (fun bm0 =>
+        (pair_args_helper (fun g1 => .. (pair_args_helper (fun g2 (_:unit) =>
+         fun bm hm => crashed%pred)) .. )))))
+  (at level 9, elem at level 0, rest at level 0,
+   g1 closed binder, g2 closed binder,
+   l1 closed binder, l2 closed binder,
+   body at level 9).
